[lf] wip.

aneris/examples/reliable_communication/lib/mt_server/proof/mt_server_proof.v
@@ -53,9 +53,8 @@ Section MTS_proof_of_code.
   Context `{SnRes : !SessionResources MT_UP}.
   Context `{HspecS : !Reliable_communication_Specified_API_session cmh}.
   Context `{HspecN : !Reliable_communication_Specified_API_network MT_UP SnRes}.
-  Context `{!MTS_spec_params}.
 
-  Lemma service_loop_proof (c : val) :
+  Lemma service_loop_proof `{!MTS_spec_params} (c : val) :
     {{{ is_monitor MTS_mN (ip_of_address MTS_saddr) MTS_mγ MTS_mv MTS_mR ∗
         c ↣{ ip_of_address MTS_saddr, MTS_rep_ser } iProto_dual req_prot  }}}
       service_loop c MTS_mv MTS_handler #() @[ip_of_address MTS_saddr]
@@ -83,7 +82,7 @@ Section MTS_proof_of_code.
     by iApply ("IH" with "[$Hc]").
   Qed.
 
-  Lemma wp_accept_new_connections_loop skt  :
+  Lemma wp_accept_new_connections_loop `{!MTS_spec_params} skt  :
     {{{ MTS_saddr ⤇ reserved_server_socket_interp ∗
         SrvListens skt ∗
         is_monitor MTS_mN (ip_of_address MTS_saddr) MTS_mγ MTS_mv MTS_mR }}}
@@ -111,7 +110,7 @@ Section MTS_proof_of_code.
       by wp_apply (service_loop_proof with "[$Hlk $Hc]").
   Qed.
 
-  Definition run_server_internal_spec A : iProp Σ :=
+  Definition run_server_internal_spec `{!MTS_spec_params} A : iProp Σ :=
     {{{ ⌜MTS_saddr ∈ A⌝ ∗
         fixed A ∗
         free_ports (ip_of_address MTS_saddr) {[port_of_address MTS_saddr]} ∗
@@ -128,7 +127,7 @@ Section MTS_proof_of_code.
         @[ip_of_address MTS_saddr]
     {{{ RET #(); ⌜True⌝ }}}.
 
-  Lemma run_server_internal_spec_holds A : ⊢ run_server_internal_spec A.
+  Lemma run_server_internal_spec_holds `{!MTS_spec_params} A : ⊢ run_server_internal_spec A.
   Proof.
     iIntros (Φ) "!#".
     iIntros "Hres HΦ".
@@ -215,22 +214,22 @@ Section MTS_proof_of_code.
 
 End MTS_proof_of_code.
 
-From aneris.examples.reliable_communication.lib.mt_server.spec Require Import api_spec.
+From aneris.examples.reliable_communication.lib.mt_server.spec
+     Require Import api_spec.
 
 Section MTS_proof_of_init.
   Context `{!anerisG Mdl Σ}.
   Context `{!lockG Σ}.
   Context `{MTU : !MTS_user_params}.
   Context `{!Reliable_communication_init}.
-  (* Context `{!MTS_spec_params}. *)
 
   Lemma MTS_init_setup_holds (E : coPset) :
     ↑MTS_mN ⊆ E →
     True ⊢ |={E}=> ∃ (srv_si : message → iProp Σ) (SrvInit : iProp Σ),
     SrvInit ∗
-    ∀ (MTS : @MTS_spec_params _ _ _ _ MTU),
-      (∀ A, run_server_spec SrvInit srv_si A) ∗
-      (∀ A sa, init_client_proxy_spec srv_si A sa).
+    (∀ (MTS : @MTS_spec_params _ _ _ _ MTU) A,
+       run_server_spec SrvInit srv_si A) ∗
+    (∀ A sa, init_client_proxy_spec srv_si A sa).
   Proof.
     iIntros (HE _).
     iMod (Reliable_communication_init_setup E MT_UP HE $! ⊤)
@@ -246,12 +245,12 @@ Section MTS_proof_of_init.
     iExists reserved_server_socket_interp, SrvInit.
     iFrame.
     iModIntro.
-    iIntros (MTS).
     iSplitL.
-    - iIntros (A Φ) "!#".
+    - iIntros (MTS A Φ) "!#".
       iIntros "(#Hsi & HinA & Hf & Hmh & Hfp & Hinit & #Hmon) HΦ".
       iDestruct run_server_internal_spec_holds as "#HserviceSpec".
-      iApply ("HserviceSpec" with "[$HinA $Hf $Hfp $Hsi $Hmon $Hmh $Hinit][$]").
+      iApply ("HserviceSpec" with
+               "[$HinA $Hf $Hfp $Hsi $Hmon $Hmh $Hinit][$]").
       Unshelve.
       + done.
       + split; done.
@@ -278,9 +277,10 @@ Section MTS_proof_of_the_init_class.
   Global Instance mts_init : MTS_init.
   Proof.
     split. iIntros (E MTU HE _).
-    iMod (MTS_init_setup_holds E HE $! ⊤) as (srv_si SrvInit) "Hinit".
+    iMod (MTS_init_setup_holds E HE $! ⊤)
+      as (srv_si SrvInit) "(Hinit & Hspecs)".
     iModIntro.
-    iExists _, _.
+    iExists _, SrvInit.
     iFrame.
     Unshelve. done.
   Qed.
