aneris/examples/reliable_communication/lib/repdb/proof/leader/proof_of_followers_handler.v
@@ -1,0 +1,62 @@
+From iris.algebra Require Import agree auth excl gmap dfrac.
+From iris.algebra.lib Require Import mono_list.
+From iris.base_logic Require Import invariants.
+From iris.bi.lib Require Import fractional.
+From iris.proofmode Require Import tactics coq_tactics reduction spec_patterns.
+From aneris.lib Require Import gen_heap_light.
+From aneris.aneris_lang Require Import lang resources inject tactics proofmode.
+From aneris.aneris_lang.lib Require Import list_proof monitor_proof lock_proof map_proof.
+From aneris.aneris_lang.lib.serialization Require Import serialization_proof.
+From aneris.aneris_lang.program_logic Require Import aneris_lifting.
+From aneris.aneris_lang.program_logic Require Import aneris_weakestpre.
+From aneris.examples.reliable_communication.prelude Require Import ser_inj.
+From aneris.examples.reliable_communication.lib.mt_server Require Import user_params.
+From aneris.examples.reliable_communication.lib.repdb Require Import repdb_code model.
+From aneris.examples.reliable_communication.lib.repdb.spec Require Import db_params events.
+From aneris.examples.reliable_communication.lib.repdb.resources
+     Require Import ras resources_def resources_global_inv resources_local_inv.
+From aneris.examples.reliable_communication.lib.repdb.proof
+     Require Import log_proof repdb_serialization.
+From aneris.examples.reliable_communication.lib.repdb.proof.leader
+     Require Import followers_mt_user_params.
+
+Import gen_heap_light.
+Import lock_proof.
+
+Section Followers_MT_spec_params.
+
+  Context `{!anerisG Mdl Σ, !DB_params, !IDBG Σ}.
+  Context (γL γM : gname).
+  Context (mγ : gname) (mv : val) (logFLoc : loc).
+
+  Notation MTU_F := (follower_handler_user_params γL γM).
+
+
+  Definition handler_cloj : val :=
+    λ: "mv" "reqv", follower_request_handler #logFLoc "mv" "reqv".
+
+  Lemma follower_request_handler_spec  :
+    ∀ reqv reqd,
+    {{{ is_monitor (DB_InvName .@ "leader_secondary")
+                  (ip_of_address MTU_F.(MTS_saddr)) mγ mv
+                   (leader_local_secondary_inv_def γL logFLoc) ∗
+        lock_proof.locked mγ ∗ (leader_local_secondary_inv_def γL logFLoc) ∗
+        MTU_F.(MTS_handler_pre) reqv reqd }}}
+      handler_cloj mv reqv @[ip_of_address MTU_F.(MTS_saddr)]
+    {{{ repv repd, RET repv;
+        ⌜Serializable rep_l2f_serialization repv⌝ ∗
+        lock_proof.locked mγ ∗ (leader_local_secondary_inv_def γL logFLoc) ∗
+        MTU_F.(MTS_handler_post) repv reqd repd }}}.
+  Proof.
+  Admitted.
+
+  Global Instance follower_handler_spec_params :  @MTS_spec_params _ _ _ _ MTU_F :=
+    {|
+      MTS_mR := (leader_local_secondary_inv_def γL logFLoc);
+      MTS_mγ := mγ;
+      MTS_mv := mv;
+      MTS_handler := handler_cloj;
+      MTS_handler_spec := follower_request_handler_spec;
+    |}.
+
+End Followers_MT_spec_params.
